\begin{slide}
\Large
\pagestyle{headings}
\sf
\header{Solution via normal equations}
Linear fit $\rightarrow$ determines estimator for $\vec{a}$
\[ \chi^2 = (\vec{y} - A\vec{a})^{t} V^{-1} 
            (\vec{y} - A\vec{a}) \]
\[Min. \chi^2 \;\rightarrow \;\frac{d\chi^2}{d\vec{a}^{\,t}}  = 0 \]
\[ \rightarrow \;-2 A^t V^{-1} (\vec{y} - A \vec{a}) = 0
\]
\[ \rightarrow \; A^t V^{-1} A \vec{a} = A^{t} V^{-1} \vec{y} \]

\noindent
{\em Side remark: why can't we just set: 
$\vec{y} = A \vec{a}$ ??? Because 
$\vec{y}$ has dimension
$n$ and $\vec{a}$ has dimension $m$ !!!
}
\noindent
\underline{Solution:}
\[ 
\begin{array}{||lll||} 
\hline
\hline
\vec{a} &  = &   (A^t V^{-1} A)^{-1} A^t V^{-1} \vec{y}  \\
 & = & H^{-1} A^t V^{-1} \vec{y} \\
 & = & U A^t V^{-1} \vec{y} \\
 & & \mbox{with}\; U= H^{-1} = Cov(a) \\ 
\hline
\hline
\end{array}
\quad
\mbox{\blue \em Normal equations}
\]
%
%
\end{slide} 

